word_lib: apply changes from afp-2025
Signed-off-by: Gerwin Klein <gerwin.klein@proofcraft.systems>

lib/Word_Lib/Rsplit.thy
@@ -2,6 +2,7 @@
  * Copyright Data61, CSIRO (ABN 41 687 119 230)
  *
  * SPDX-License-Identifier: BSD-2-Clause
+Proofs tidied by LCP, 2024-09
  *)
 
 (* Author: Jeremy Dawson and Gerwin Klein, NICTA *)
@@ -9,8 +10,253 @@
 section \<open>Splitting words into lists\<close>
 
 theory Rsplit
-  imports "HOL-Library.Word" More_Word Bits_Int
+  imports More_Word Bit_Shifts_Infix_Syntax
+
+
 begin
+
+lemmas th_if_simp1 = if_split [where P = "(=) l", THEN iffD1, THEN conjunct1, THEN mp] for l
+lemmas th_if_simp2 = if_split [where P = "(=) l", THEN iffD1, THEN conjunct2, THEN mp] for l
+
+
+definition bin_split :: \<open>nat \<Rightarrow> int \<Rightarrow> int \<times> int\<close>
+  where [simp]: \<open>bin_split n k = (drop_bit n k, take_bit n k)\<close>
+
+lemma [code]:
+  "bin_split (Suc n) w = (let (w1, w2) = bin_split n (w div 2) in (w1, of_bool (odd w) + 2 * w2))"
+  "bin_split 0 w = (w, 0)"
+  by (simp_all add: drop_bit_Suc take_bit_Suc mod_2_eq_odd)
+
+fun bin_rsplit_aux :: "nat \<Rightarrow> nat \<Rightarrow> int \<Rightarrow> int list \<Rightarrow> int list"
+  where "bin_rsplit_aux n m c bs =
+    (if m = 0 \<or> n = 0 then bs
+     else
+      let (a, b) = bin_split n c
+      in bin_rsplit_aux n (m - n) a (b # bs))"
+
+definition bin_rsplit :: "nat \<Rightarrow> nat \<times> int \<Rightarrow> int list"
+  where "bin_rsplit n w = bin_rsplit_aux n (fst w) (snd w) []"
+
+fun bin_rsplitl_aux :: "nat \<Rightarrow> nat \<Rightarrow> int \<Rightarrow> int list \<Rightarrow> int list"
+  where "bin_rsplitl_aux n m c bs =
+    (if m = 0 \<or> n = 0 then bs
+     else
+      let (a, b) = bin_split (min m n) c
+      in bin_rsplitl_aux n (m - n) a (b # bs))"
+
+definition bin_rsplitl :: "nat \<Rightarrow> nat \<times> int \<Rightarrow> int list"
+  where "bin_rsplitl n w = bin_rsplitl_aux n (fst w) (snd w) []"
+
+declare bin_rsplit_aux.simps [simp del]
+declare bin_rsplitl_aux.simps [simp del]
+
+lemma bin_nth_split:
+  "bin_split n c = (a, b) \<Longrightarrow>
+    (\<forall>k. (bit :: int \<Rightarrow> nat \<Rightarrow> bool) a k = (bit :: int \<Rightarrow> nat \<Rightarrow> bool) c (n + k)) \<and>
+    (\<forall>k. (bit :: int \<Rightarrow> nat \<Rightarrow> bool) b k = (k < n \<and> (bit :: int \<Rightarrow> nat \<Rightarrow> bool) c k))"
+  by (force simp add: bit_simps)
+
+lemma split_bintrunc: "bin_split n c = (a, b) \<Longrightarrow> b = (take_bit :: nat \<Rightarrow> int \<Rightarrow> int) n c"
+  by simp
+
+lemma bin_cat_split: "bin_split n w = (u, v) \<Longrightarrow> w = (\<lambda>k n l. concat_bit n l k) u n v"
+  using bits_ident [of n w]
+  by (metis Pair_inject add.commute bin_split_def concat_bit_eq concat_bit_take_bit_eq)
+
+lemma bin_split_cat: "bin_split n ((\<lambda>k n l. concat_bit n l k) v n w) = (v, (take_bit :: nat \<Rightarrow> int \<Rightarrow> int) n w)"
+  by (metis bin_cat_split bin_split_def concat_bit_eq_iff concat_bit_take_bit_eq)
+
+lemma bin_split_zero [simp]: "bin_split n 0 = (0, 0)"
+  by simp
+
+lemma bin_split_minus1 [simp]:
+  "bin_split n (- 1) = (- 1, (take_bit :: nat \<Rightarrow> int \<Rightarrow> int) n (- 1))"
+  by simp
+
+lemma bin_split_trunc:
+  "bin_split (min m n) c = (a, b) \<Longrightarrow>
+    bin_split n ((take_bit :: nat \<Rightarrow> int \<Rightarrow> int) m c) = ((take_bit :: nat \<Rightarrow> int \<Rightarrow> int) (m - n) a, b)"
+  by (cases \<open>n \<le> m\<close>) (auto simp add: drop_bit_take_bit ac_simps)+
+
+lemma bin_split_trunc1:
+  "bin_split n c = (a, b) \<Longrightarrow>
+    bin_split n ((take_bit :: nat \<Rightarrow> int \<Rightarrow> int) m c) = ((take_bit :: nat \<Rightarrow> int \<Rightarrow> int) (m - n) a, (take_bit :: nat \<Rightarrow> int \<Rightarrow> int) m b)"
+  by (force simp add: drop_bit_take_bit ac_simps)
+
+lemma bin_split_num: "bin_split n b = (b div 2 ^ n, b mod 2 ^ n)"
+  by (simp add: drop_bit_eq_div take_bit_eq_mod)
+
+lemmas bin_rsplit_aux_simps = bin_rsplit_aux.simps bin_rsplitl_aux.simps
+lemmas rsplit_aux_simps = bin_rsplit_aux_simps
+
+lemmas rsplit_aux_simp1s = rsplit_aux_simps [THEN th_if_simp1]
+
+lemmas rsplit_aux_simp2ls = rsplit_aux_simps [THEN th_if_simp2]
+\<comment> \<open>these safe to \<open>[simp add]\<close> as require calculating \<open>m - n\<close>\<close>
+lemmas bin_rsplit_aux_simp2s [simp] = rsplit_aux_simp2ls [unfolded Let_def]
+lemmas rbscl = bin_rsplit_aux_simp2s (2)
+
+lemmas rsplit_aux_0_simps [simp] =
+  rsplit_aux_simp1s [OF disjI1] rsplit_aux_simp1s [OF disjI2]
+
+lemma bin_rsplit_aux_append: "bin_rsplit_aux n m c (bs @ cs) = bin_rsplit_aux n m c bs @ cs"
+proof (induct n m c bs rule: bin_rsplit_aux.induct)
+  case (1 n m c bs)
+  then show ?case
+    by (simp add: rsplit_aux_simps)
+qed
+
+lemma bin_rsplitl_aux_append: "bin_rsplitl_aux n m c (bs @ cs) = bin_rsplitl_aux n m c bs @ cs"
+proof (induct n m c bs rule: bin_rsplitl_aux.induct)
+  case (1 n m c bs)
+  then show ?case
+    by (simp add: rsplit_aux_simps)
+qed
+
+lemmas rsplit_aux_apps [where bs = "[]"] =
+  bin_rsplit_aux_append bin_rsplitl_aux_append
+
+lemmas rsplit_def_auxs = bin_rsplit_def bin_rsplitl_def
+
+lemmas rsplit_aux_alts = rsplit_aux_apps
+  [unfolded append_Nil rsplit_def_auxs [symmetric]]
+
+lemma bin_split_minus: "0 < n \<Longrightarrow> bin_split (Suc (n - 1)) w = bin_split n w"
+  by auto
+
+lemma bin_split_pred_simp [simp]:
+  "(0::nat) < numeral bin \<Longrightarrow>
+    bin_split (numeral bin) w =
+      (let (w1, w2) = bin_split (numeral bin - 1) ((\<lambda>k::int. k div 2) w)
+       in (w1, of_bool (odd w) + 2 * w2))"
+  by (simp add: take_bit_rec drop_bit_rec mod_2_eq_odd)
+
+lemma bin_rsplit_aux_simp_alt:
+  "bin_rsplit_aux n m c bs =
+    (if m = 0 \<or> n = 0 then bs
+     else let (a, b) = bin_split n c in bin_rsplit n (m - n, a) @ b # bs)"
+  apply (simp add: rsplit_def_auxs)
+  using rsplit_aux_alts(1) by blast
+
+lemmas bin_rsplit_simp_alt =
+  trans [OF bin_rsplit_def bin_rsplit_aux_simp_alt]
+
+lemmas bthrs = bin_rsplit_simp_alt [THEN [2] trans]
+
+lemma bin_rsplit_size_sign':
+  "n > 0 \<Longrightarrow> rev sw = bin_rsplit n (nw, w) \<Longrightarrow> v\<in>set sw \<Longrightarrow> (take_bit :: nat \<Rightarrow> int \<Rightarrow> int) n v = v"
+proof (induct sw arbitrary: nw w)
+  case Nil
+  then show ?case by auto
+next
+  case (Cons a sw)
+  then show ?case
+    by (force dest: bthrs split: if_split_asm)
+qed
+
+lemmas bin_rsplit_size_sign = bin_rsplit_size_sign' [OF asm_rl
+  rev_rev_ident [THEN trans] set_rev [THEN equalityD2 [THEN subsetD]]]
+
+lemma bin_nth_rsplit:
+  "\<lbrakk>n > 0; m < n; rev sw = bin_rsplit n (nw, w); k < size sw\<rbrakk>
+   \<Longrightarrow> (bit :: int \<Rightarrow> nat \<Rightarrow> bool) (sw ! k) m = (bit :: int \<Rightarrow> nat \<Rightarrow> bool) w (k * n + m)"
+proof (induct sw arbitrary: w k nw)
+  case Nil
+  then show ?case by auto
+next
+  case (Cons a sw w k nw)
+  have "bit ((take_bit n w # sw) ! k) m = bit w (k * n + m)"
+    if "rev sw = bin_rsplit n (nw - n, drop_bit n w)"
+    using that Cons
+    by (cases k) (simp_all add: bit_take_bit_iff bit_drop_bit_eq ac_simps)
+  with Cons show ?case
+    by (force dest: bthrs split: if_split_asm)
+qed
+
+lemma bin_rsplit_all: "0 < nw \<Longrightarrow> nw \<le> n \<Longrightarrow> bin_rsplit n (nw, w) = [(take_bit :: nat \<Rightarrow> int \<Rightarrow> int) n w]"
+  by (auto simp: bin_rsplit_def rsplit_aux_simp2ls split: prod.split dest!: split_bintrunc)
+
+lemma bin_rsplit_l [rule_format]:
+  "bin_rsplitl n (m, bin) = bin_rsplit n (m, (take_bit :: nat \<Rightarrow> int \<Rightarrow> int) m bin)"
+  using wf_less_than
+proof (induct m arbitrary: bin rule: wf_induct_rule)
+  case (less m)
+  then have "bin_rsplitl_aux n (m - n) (drop_bit (min m n) bin) [] 
+           = bin_rsplit_aux n (m - n) (drop_bit n (take_bit m bin)) []"
+    if "0 < m" and "0 < n"
+    using that  by (simp add: drop_bit_take_bit min_def rsplit_def_auxs)
+  then show ?case
+    unfolding bin_rsplitl_def bin_rsplit_def 
+    apply (subst bin_rsplitl_aux.simps)
+    apply (clarsimp simp: Let_def ac_simps split: prod.split)
+    by (metis rsplit_aux_alts)
+qed
+
+lemma bin_rsplit_lemma: "sc - n + (n + lb * n) \<le> m * n \<longleftrightarrow> sc + lb * n \<le> m * n"
+  if "0 < sc" for sc m n lb :: nat
+proof (cases "sc \<ge> n")
+  case False
+  with that show ?thesis
+    using linorder_le_less_linear [of m lb] 
+    by (smt (verit, ccfv_SIG) Nat.le_diff_conv2 add_leD2 diff_is_0_eq' le0 mult_Suc mult_le_cancel2 not_less_eq_eq order_trans)
+qed auto
+
+lemma bin_rsplit_aux_len_le:
+  "n \<noteq> 0 \<Longrightarrow> ws = bin_rsplit_aux n nw w bs \<Longrightarrow>
+    length ws \<le> m \<longleftrightarrow> nw + length bs * n \<le> m * n"
+proof (induct n nw w bs rule: bin_rsplit_aux.induct)
+  case (1 n m c bs)
+  then show ?case
+    by (simp add: bin_rsplit_aux_simps bin_rsplit_lemma Let_def)
+qed
+
+lemma bin_rsplit_len_le: "n \<noteq> 0 \<longrightarrow> ws = bin_rsplit n (nw, w) \<longrightarrow> length ws \<le> m \<longleftrightarrow> nw \<le> m * n"
+  by (auto simp: bin_rsplit_def bin_rsplit_aux_len_le)
+
+lemma bin_rsplit_aux_len:
+  "n \<noteq> 0 \<Longrightarrow> length (bin_rsplit_aux n nw w cs) = (nw + n - 1) div n + length cs"
+proof (induct n nw w cs rule: bin_rsplit_aux.induct)
+  case (1 n m c bs)
+  have "\<lbrakk>0 < n; 0 < m\<rbrakk> \<Longrightarrow> Suc ((m - n + n - Suc 0) div n) = (m + n - Suc 0) div n"
+    using div_if by force
+  with 1 show ?case
+    by (auto simp: bin_rsplit_aux.simps)
+qed
+
+lemma bin_rsplit_len: "n \<noteq> 0 \<Longrightarrow> length (bin_rsplit n (nw, w)) = (nw + n - 1) div n"
+  by (auto simp: bin_rsplit_def bin_rsplit_aux_len)
+
+lemma bin_rsplit_aux_len_indep:
+  "n \<noteq> 0 \<Longrightarrow> length bs = length cs \<Longrightarrow>
+    length (bin_rsplit_aux n nw v bs) =
+    length (bin_rsplit_aux n nw w cs)"
+proof (induct n nw w cs arbitrary: v bs rule: bin_rsplit_aux.induct)
+  case (1 n m w cs v bs)
+  show ?case
+  proof (cases "m = 0")
+    case True
+    with \<open>length bs = length cs\<close> show ?thesis by simp
+  next
+    case False
+    from "1.hyps" [of \<open>bin_split n w\<close> \<open>drop_bit n w\<close> \<open>take_bit n w\<close>] \<open>m \<noteq> 0\<close> \<open>n \<noteq> 0\<close>
+    have hyp: "\<And>v bs. length bs = Suc (length cs) \<Longrightarrow>
+      length (bin_rsplit_aux n (m - n) v bs) =
+      length (bin_rsplit_aux n (m - n) (drop_bit n w) (take_bit n w # cs))"
+      using bin_rsplit_aux_len by fastforce
+    from \<open>length bs = length cs\<close> \<open>n \<noteq> 0\<close> show ?thesis
+      by (auto simp add: bin_rsplit_aux_simp_alt Let_def bin_rsplit_len split: prod.split)
+  qed
+qed
+
+lemma bin_rsplit_len_indep:
+  "n \<noteq> 0 \<Longrightarrow> length (bin_rsplit n (nw, v)) = length (bin_rsplit n (nw, w))"
+  using bin_rsplit_len by presburger
+
+lemma split_uint_lem: "bin_split n (uint w) = (a, b) \<Longrightarrow>
+    a = take_bit (LENGTH('a) - n) a \<and> b = take_bit (LENGTH('a)) b"
+  for w :: "'a::len word"
+  by transfer (simp add: drop_bit_take_bit ac_simps)
+
 
 definition word_rsplit :: "'a::len word \<Rightarrow> 'b::len word list"
   where "word_rsplit w = map word_of_int (bin_rsplit LENGTH('b) (LENGTH('a), uint w))"
@@ -30,52 +276,34 @@ text \<open>
   and therefore of the same length, as the original word.\<close>
 
 lemma word_rsplit_same: "word_rsplit w = [w]"
-  apply (simp add: word_rsplit_def bin_rsplit_all)
-  apply transfer
-  apply simp
-  done
+  by (simp add: word_rsplit_def bintr_uint bin_rsplit_all)
 
 lemma word_rsplit_empty_iff_size: "word_rsplit w = [] \<longleftrightarrow> size w = 0"
   by (simp add: word_rsplit_def bin_rsplit_def word_size bin_rsplit_aux_simp_alt Let_def
       split: prod.split)
 
-lemma test_bit_rsplit:
-  "sw = word_rsplit w \<Longrightarrow> m < size (hd sw) \<Longrightarrow>
-    k < length sw \<Longrightarrow> bit (rev sw ! k) m = bit w (k * size (hd sw) + m)"
-  for sw :: "'a::len word list"
-  apply (unfold word_rsplit_def word_test_bit_def)
-  apply (rule trans)
-   apply (rule_tac f = "\<lambda>x. bit x m" in arg_cong)
-   apply (rule nth_map [symmetric])
-   apply simp
-  apply (rule bin_nth_rsplit)
-     apply simp_all
-  apply (simp add : word_size rev_map)
-  apply (rule trans)
-   defer
-   apply (rule map_ident [THEN fun_cong])
-  apply (rule refl [THEN map_cong])
-  apply (simp add: unsigned_of_int take_bit_int_eq_self_iff)
-  using bin_rsplit_size_sign take_bit_int_eq_self_iff by blast
+lemma test_bit_rsplit [OF refl]:
+  fixes sw :: "'a::len word list"
+  assumes "sw = word_rsplit w" "m < size (hd sw)" "k < length sw"
+    shows "bit (rev sw ! k) m = bit w (k * size (hd sw) + m)"
+proof -
+  have "bit (rev sw ! k) m = bit (map uint (rev sw) ! k) m"
+    by (simp add: assms(3) word_test_bit_def)
+  also have "... = bit (uint w) (k * size (hd sw) + m)"
+    using assms  
+    by (simp add: bin_nth_rsplit bit_take_bit_iff rev_map unsigned_of_int
+        word_rsplit_def word_size)
+  also have "... = bit w (k * size (hd sw) + m)"
+    by (simp add: test_bit_def')
+  finally show ?thesis .
+qed
 
 lemma test_bit_rsplit_alt:
   \<open>bit ((word_rsplit w  :: 'b::len word list) ! i) m \<longleftrightarrow>
     bit w ((length (word_rsplit w :: 'b::len word list) - Suc i) * size (hd (word_rsplit w :: 'b::len word list)) + m)\<close>
   if \<open>i < length (word_rsplit w :: 'b::len word list)\<close> \<open>m < size (hd (word_rsplit w :: 'b::len word list))\<close> \<open>0 < length (word_rsplit w :: 'b::len word list)\<close>
   for w :: \<open>'a::len word\<close>
-  apply (rule trans)
-   apply (rule test_bit_cong)
-   apply (rule rev_nth [of _ \<open>rev (word_rsplit w)\<close>, simplified rev_rev_ident])
-  apply simp
-   apply (rule that(1))
-  apply simp
-  apply (rule test_bit_rsplit)
-    apply (rule refl)
-  apply (rule asm_rl)
-   apply (rule that(2))
-  apply (rule diff_Suc_less)
-  apply (rule that(3))
-  done
+  by (metis diff_Suc_less length_rev rev_nth rev_rev_ident test_bit_rsplit that)
 
 lemma word_rsplit_len_indep [OF refl refl refl refl]:
   "[u,v] = p \<Longrightarrow> [su,sv] = q \<Longrightarrow> word_rsplit u = su \<Longrightarrow>
@@ -107,14 +335,19 @@ lemmas tdle = times_div_less_eq_dividend
 lemmas dtle = xtrans(4) [OF tdle mult.commute]
 
 lemma word_rcat_rsplit: "word_rcat (word_rsplit w) = w"
-  apply (rule word_eqI)
-  apply (clarsimp simp: test_bit_rcat word_size)
-  apply (subst refl [THEN test_bit_rsplit])
-    apply (simp_all add: word_size
-      refl [THEN length_word_rsplit_size [simplified not_less [symmetric], simplified]])
-   apply safe
-   apply (erule xtrans(7), rule dtle)+
-  done
+proof (rule word_eqI)
+  fix n 
+  assume "n < size (word_rcat (word_rsplit w::'b word list)::'a word)"
+  then have n: "n < LENGTH('a)"
+    by (simp add: word_size)
+  show "bit (word_rcat (word_rsplit w::'b word list)::'a word) n = bit w n"
+  proof -
+    have "\<forall>k. k * (n div k) < LENGTH('a)"
+      by (metis (no_types) n order_le_less_trans times_div_less_eq_dividend)
+    with n show ?thesis
+      by (simp add: length_word_rsplit_lt_size mult.commute test_bit_rcat test_bit_rsplit word_size)
+  qed
+qed
 
 lemma size_word_rsplit_rcat_size:
   "word_rcat ws = frcw \<Longrightarrow> size frcw = length ws * LENGTH('a)
@@ -122,42 +355,43 @@ lemma size_word_rsplit_rcat_size:
   for ws :: "'a::len word list" and frcw :: "'b::len word"
   by (cases \<open>LENGTH('a)\<close>) (simp_all add: word_size length_word_rsplit_exp_size' div_nat_eqI)
 
-lemma word_rsplit_rcat_size [OF refl]:
-  "word_rcat ws = frcw \<Longrightarrow>
-    size frcw = length ws * LENGTH('a) \<Longrightarrow> word_rsplit frcw = ws"
-  for ws :: "'a::len word list"
-  apply (frule size_word_rsplit_rcat_size, assumption)
-  apply (clarsimp simp add : word_size)
-  apply (rule nth_equalityI, assumption)
-  apply clarsimp
-  apply (rule word_eqI [rule_format])
-  apply (rule trans)
-   apply (rule test_bit_rsplit_alt)
-     apply (clarsimp simp: word_size)+
-  apply (rule trans)
-   apply (rule test_bit_rcat [OF refl refl])
-  apply (simp add: word_size)
-  apply (subst rev_nth)
-   apply arith
-  apply (simp add: le0 [THEN [2] xtrans(7), THEN diff_Suc_less])
-  apply safe
-  apply (simp add: diff_mult_distrib)
-   apply (cases "size ws")
-    apply simp_all
-  done
+lemma word_rsplit_rcat_size:
+  fixes ws :: "'a::len word list"
+  defines "frcw \<equiv> word_rcat ws"
+  assumes "size frcw = length ws * LENGTH('a)" 
+  shows "word_rsplit frcw = ws"
+proof (intro nth_equalityI word_eqI)
+  show "length (word_rsplit frcw::'a word list) = length ws"
+    using size_word_rsplit_rcat_size assms by blast
+next
+  fix i n
+  assume \<section>: "i < length (word_rsplit frcw::'a word list)" 
+    "n < size (word_rsplit frcw ! i::'a word)"
+  then have n: "n < LENGTH('a)"
+    by (simp add: word_size)
+  then have *: "(length ws - Suc i) * LENGTH('a) + n < length ws * LENGTH('a)" 
+    using assms div_eq_0_iff td_gal_lt by fastforce
+  have i: "i < length ws"
+    by (metis \<section> assms(2) length_word_rsplit_even_size)
+  then have **: "bit (word_rcat ws :: 'b word) ((length ws - Suc i) * LENGTH('a) + n) 
+      = bit (ws ! i) n"
+    using n assms * 
+    by (auto simp add: test_bit_rcat [OF refl refl] rev_nth word_size)
+  then show "bit (word_rsplit frcw ! i::'a word) n = bit (ws ! i) n"
+    using n i assms test_bit_rsplit_alt
+    by (metis (mono_tags, lifting) len_gt_0 length_word_rsplit_even_size 
+         word_size zero_less_mult_pos2)
+qed
 
 lemma word_rsplit_upt:
-  "\<lbrakk> size x = LENGTH('a :: len) * n; n \<noteq> 0 \<rbrakk>
-    \<Longrightarrow> word_rsplit x = map (\<lambda>i. ucast (x >> (i * LENGTH('a))) :: 'a word) (rev [0 ..< n])"
-  apply (subgoal_tac "length (word_rsplit x :: 'a word list) = n")
-   apply (rule nth_equalityI, simp)
-   apply (intro allI word_eqI impI)
-   apply (simp add: test_bit_rsplit_alt word_size)
-   apply (simp add: nth_ucast bit_simps rev_nth field_simps)
-  apply (simp add: length_word_rsplit_exp_size word_size)
-  apply (subst diff_add_assoc)
-   apply (simp flip: less_eq_Suc_le)
-  apply simp
-  done
-
+  assumes "size x = LENGTH('a :: len) * n" and "n \<noteq> 0"
+  shows "word_rsplit x = map (\<lambda>i. ucast (x >> (i * LENGTH('a))) :: 'a word) (rev [0 ..< n])"
+proof -
+  have "length (word_rsplit x :: 'a word list) = n"
+    by (simp add: assms length_word_rsplit_even_size)
+  then show ?thesis
+    using assms
+    by (intro nth_equalityI word_eqI) (auto simp add: test_bit_rsplit_alt word_size bit_simps rev_nth)
+qed
+    
 end
