lib/Word_Lib/Bitwise.thy
@@ -10,6 +10,7 @@ theory Bitwise
     More_Arithmetic
     Reversed_Bit_Lists
     Bit_Shifts_Infix_Syntax
+
 begin
 
 text \<open>Helper constants used in defining addition\<close>
@@ -46,14 +47,7 @@ lemma bl_word_sub: "to_bl (x - y) = to_bl (x + (- y))"
   by simp
 
 lemma rbl_word_1: "rev (to_bl (1 :: 'a::len word)) = takefill False (LENGTH('a)) [True]"
-  apply (rule_tac s="rev (to_bl (word_succ (0 :: 'a word)))" in trans)
-   apply simp
-  apply (simp only: rtb_rbl_ariths(1)[OF refl])
-  apply simp
-  apply (case_tac "LENGTH('a)")
-   apply simp
-  apply (simp add: takefill_alt)
-  done
+  by (metis rev_rev_ident rev_singleton_conv word_1_bl word_rev_tf)
 
 lemma rbl_word_if: "rev (to_bl (if P then x else y)) = map2 (If P) (rev (to_bl x)) (rev (to_bl y))"
   by (simp add: split_def)
@@ -67,21 +61,21 @@ lemma rbl_add_suc_carry_fold:
   "length xs = length ys \<Longrightarrow>
     \<forall>car. (if car then rbl_succ else id) (rbl_add xs ys) =
       (foldr (\<lambda>(x, y) res car. xor3 x y car # res (carry x y car)) (zip xs ys) (\<lambda>_. [])) car"
-  apply (erule list_induct2)
-   apply simp
-  apply (simp only: rbl_add_carry_Cons)
-  apply simp
-  done
+proof (induction rule: list_induct2)
+  case Nil
+  then show ?case by simp
+next
+  case (Cons x xs y ys)
+  then show ?case
+    using rbl_add_carry_Cons by auto
+qed
 
 lemma to_bl_plus_carry:
   "to_bl (x + y) =
     rev (foldr (\<lambda>(x, y) res car. xor3 x y car # res (carry x y car))
       (rev (zip (to_bl x) (to_bl y))) (\<lambda>_. []) False)"
   using rbl_add_suc_carry_fold[where xs="rev (to_bl x)" and ys="rev (to_bl y)"]
-  apply (simp add: word_add_rbl[OF refl refl])
-  apply (drule_tac x=False in spec)
-  apply (simp add: zip_rev)
-  done
+  by (smt (verit) id_apply length_rev word_add_rbl word_rotate.lbl_lbl zip_rev)
 
 definition "rbl_plus cin xs ys =
   foldr (\<lambda>(x, y) res car. xor3 x y car # res (carry x y car)) (zip xs ys) (\<lambda>_. []) cin"
@@ -118,17 +112,11 @@ lemma rbl_word_cat:
 lemma rbl_word_slice:
   "rev (to_bl (slice n w :: 'a::len word)) =
     takefill False (LENGTH('a)) (drop n (rev (to_bl w)))"
-  apply (simp add: slice_take word_rev_tf rev_take)
-  apply (cases "n < LENGTH('b)", simp_all)
-  done
+  by (simp add: drop_rev slice_take word_rev_tf)
 
 lemma rbl_word_ucast:
   "rev (to_bl (ucast x :: 'a::len word)) = takefill False (LENGTH('a)) (rev (to_bl x))"
-  apply (simp add: to_bl_ucast takefill_alt)
-  apply (simp add: rev_drop)
-  apply (cases "LENGTH('a) < LENGTH('b)")
-   apply simp_all
-  done
+  by (simp add: takefill_alt ucast_bl word_rev_tf)
 
 lemma rbl_shiftl:
   "rev (to_bl (w << n)) = takefill False (size w) (replicate n False @ rev (to_bl w))"
@@ -156,48 +144,46 @@ lemma takefill_last_simps:
 
 lemma rbl_sshiftr:
   "rev (to_bl (w >>> n)) = takefill_last False (size w) (drop_nonempty False n (rev (to_bl w)))"
-  apply (cases "n < size w")
-   apply (simp add: bl_sshiftr takefill_last_def word_size
-      takefill_alt rev_take last_rev
-      drop_nonempty_def)
-  apply (subgoal_tac "(w >>> n) = of_bl (replicate (size w) (msb w))")
+proof (cases "n < size w")
+  case True
+  then show ?thesis
+    by (simp add: bl_sshiftr takefill_last_def word_size takefill_alt
+           rev_take last_rev drop_nonempty_def)    
+next
+  case False
+  then have \<section>: "(w >>> n) = of_bl (replicate (size w) (msb w))"
+    by (intro word_eqI) (simp add: bit_simps word_size msb_nth)
+  with False show ?thesis
    apply (simp add: word_size takefill_last_def takefill_alt
-      last_rev word_msb_alt word_rev_tf
-      drop_nonempty_def take_Cons')
-   apply (case_tac "LENGTH('a)", simp_all)
-  apply (rule word_eqI)
-  apply (simp add: bit_simps word_size test_bit_of_bl
-      msb_nth)
-  done
+      last_rev word_msb_alt word_rev_tf drop_nonempty_def take_Cons')
+    by (metis Suc_pred len_gt_0 replicate_Suc)
+qed
 
 lemma nth_word_of_int:
   "bit (word_of_int x :: 'a::len word) n = (n < LENGTH('a) \<and> bit x n)"
-  apply (simp add: test_bit_bl word_size to_bl_of_bin)
-  apply (subst conj_cong[OF refl], erule bin_nth_bl)
-  apply auto
-  done
+  by (simp add: bit_word_of_int_iff)
 
 lemma nth_scast:
   "bit (scast (x :: 'a::len word) :: 'b::len word) n =
     (n < LENGTH('b) \<and>
     (if n < LENGTH('a) - 1 then bit x n
      else bit x (LENGTH('a) - 1)))"
-  apply transfer
-  apply (auto simp add: bit_signed_take_bit_iff min_def)
-  done
+  by (simp add: bit_signed_iff)
 
 lemma rbl_word_scast:
   "rev (to_bl (scast x :: 'a::len word)) = takefill_last False (LENGTH('a)) (rev (to_bl x))"
-  apply (rule nth_equalityI)
-   apply (simp add: word_size takefill_last_def)
-  apply (clarsimp simp: nth_scast takefill_last_def
-      nth_takefill word_size rev_nth to_bl_nth)
+proof (rule nth_equalityI)
+  show "length (rev (to_bl (scast x::'a word))) = length (takefill_last False (len_of (TYPE('a)::'a itself)) (rev (to_bl x)))"
+    by (simp add: word_size takefill_last_def)
+next
+  fix i 
+  assume "i < length (rev (to_bl (scast x::'a word)))"
+  then show "rev (to_bl (scast x::'a word)) ! i = takefill_last False (LENGTH('a)) (rev (to_bl x)) ! i"
   apply (cases "LENGTH('b)")
-   apply simp
-  apply (clarsimp simp: less_Suc_eq_le linorder_not_less
-      last_rev word_msb_alt[symmetric]
-      msb_nth)
+     apply (auto simp: nth_scast takefill_last_def nth_takefill word_size rev_nth 
+        to_bl_nth less_Suc_eq_le last_rev msb_nth simp flip: word_msb_alt)
   done
+qed
 
 definition rbl_mul :: "bool list \<Rightarrow> bool list \<Rightarrow> bool list"
   where "rbl_mul xs ys = foldr (\<lambda>x sm. rbl_plus False (map ((\<and>) x) ys) (False # sm)) xs []"
@@ -211,12 +197,8 @@ lemma takefill_le2: "length xs \<le> n \<Longrightarrow> takefill x m (takefill 
   by (simp add: takefill_alt replicate_add[symmetric])
 
 lemma take_rbl_plus: "\<forall>n b. take n (rbl_plus b xs ys) = rbl_plus b (take n xs) (take n ys)"
-  apply (simp add: rbl_plus_def take_zip[symmetric])
-  apply (rule_tac list="zip xs ys" in list.induct)
-   apply simp
-  apply (clarsimp simp: split_def)
-  apply (case_tac n, simp_all)
-  done
+  unfolding rbl_plus_def take_zip[symmetric]
+  by (rule list.induct) (auto simp: take_Cons' split_def)
 
 lemma word_rbl_mul_induct:
   "length xs \<le> size y \<Longrightarrow>
@@ -241,15 +223,18 @@ next
   have zip_take_triv: "\<And>xs ys n. n = length ys \<Longrightarrow> zip (take n xs) ys = zip xs ys"
     by (rule nth_equalityI) simp_all
 
-  from Cons show ?case
-    apply (simp add: trans [OF of_bl_append add.commute]
-        rbl_mul_simps rbl_word_plus' distrib_right mult_bit shiftl rbl_shiftl)
-    apply (simp add: takefill_alt word_size rev_map take_rbl_plus min_def)
-    apply (simp add: rbl_plus_def)
-    apply (simp add: zip_take_triv)
-    apply (simp only: mult.commute [of _ 2] to_bl_double_eq)
-    apply (simp flip: butlast_rev add: take_butlast)
-    done
+  from Cons
+  have "rbl_plus False (map ((\<and>) z) (rev (to_bl y)))
+         (False # take (length zs) (rev (to_bl (of_bl (rev zs) * y)))) =
+        rbl_plus False
+         (take (Suc (length zs)) (map ((\<and>) z) (rev (to_bl y))))
+         (take (Suc (length zs)) (rev (to_bl (of_bl (rev zs) * y * 2))))"
+    unfolding word_size
+    by (simp add: rbl_plus_def zip_take_triv mult.commute [of _ 2] to_bl_double_eq take_butlast
+        flip: butlast_rev)
+  with Cons show ?case
+    by (simp add: trans [OF of_bl_append add.commute]
+        rbl_mul_simps rbl_word_plus' distrib_right mult_bit shiftl rev_map take_rbl_plus)
 qed
 
 lemma rbl_word_mul: "rev (to_bl (x * y)) = rbl_mul (rev (to_bl x)) (rev (to_bl y))"
@@ -269,17 +254,7 @@ lemma rev_bl_order_simps:
   "rev_bl_order F [] [] = F"
   "rev_bl_order F (x # xs) (y # ys) = rev_bl_order ((y \<and> \<not> x) \<or> ((y \<or> \<not> x) \<and> F)) xs ys"
    apply (simp_all add: rev_bl_order_def)
-  apply (rule conj_cong[OF refl])
-  apply (cases "xs = ys")
-   apply (simp add: nth_Cons')
-   apply blast
-  apply (simp add: nth_Cons')
-  apply safe
-   apply (rule_tac x="n - 1" in exI)
-   apply simp
-  apply (rule_tac x="Suc n" in exI)
-  apply simp
-  done
+  using less_Suc_eq_0_disj by fastforce
 
 lemma rev_bl_order_rev_simp:
   "length xs = length ys \<Longrightarrow>
@@ -290,10 +265,17 @@ lemma rev_bl_order_bl_to_bin:
   "length xs = length ys \<Longrightarrow>
     rev_bl_order True xs ys = (bl_to_bin (rev xs) \<le> bl_to_bin (rev ys)) \<and>
     rev_bl_order False xs ys = (bl_to_bin (rev xs) < bl_to_bin (rev ys))"
-  apply (induct xs ys rule: list_induct2)
-   apply (simp_all add: rev_bl_order_simps bl_to_bin_app_cat concat_bit_Suc)
-  apply (auto simp add: bl_to_bin_def add1_zle_eq)
-  done
+proof (induct xs ys rule: list_induct2)
+  case Nil
+  then show ?case 
+    by (auto simp: rev_bl_order_simps(1))
+next
+  case (Cons x xs y ys)
+  then show ?case 
+    apply (simp add: rev_bl_order_simps bl_to_bin_app_cat)
+    apply (auto simp add: bl_to_bin_def add1_zle_eq concat_bit_Suc)
+    done
+qed
 
 lemma word_le_rbl: "x \<le> y \<longleftrightarrow> rev_bl_order True (rev (to_bl x)) (rev (to_bl y))"
   for x y :: "'a::len word"
@@ -313,25 +295,18 @@ lemma map_last_simps:
 
 lemma word_sle_rbl:
   "x <=s y \<longleftrightarrow> rev_bl_order True (map_last Not (rev (to_bl x))) (map_last Not (rev (to_bl y)))"
-  using word_msb_alt[where w=x] word_msb_alt[where w=y]
-  apply (simp add: word_sle_msb_le word_le_rbl)
-  apply (subgoal_tac "length (to_bl x) = length (to_bl y)")
-   apply (cases "to_bl x", simp)
-   apply (cases "to_bl y", simp)
-   apply (clarsimp simp: map_last_def rev_bl_order_rev_simp)
-   apply auto
-  done
+proof -
+  have "length (to_bl x) = length (to_bl y)"
+    by auto
+  with word_msb_alt[where w=x] word_msb_alt[where w=y]
+  show ?thesis
+    unfolding word_sle_msb_le word_le_rbl
+    by (cases "to_bl x"; cases "to_bl y"; auto simp: map_last_def rev_bl_order_rev_simp)
+qed
 
 lemma word_sless_rbl:
   "x <s y \<longleftrightarrow> rev_bl_order False (map_last Not (rev (to_bl x))) (map_last Not (rev (to_bl y)))"
-  using word_msb_alt[where w=x] word_msb_alt[where w=y]
-  apply (simp add: word_sless_msb_less word_less_rbl)
-  apply (subgoal_tac "length (to_bl x) = length (to_bl y)")
-   apply (cases "to_bl x", simp)
-   apply (cases "to_bl y", simp)
-   apply (clarsimp simp: map_last_def rev_bl_order_rev_simp)
-   apply auto
-  done
+  by (metis (no_types, lifting) rev_bl_order_def signed.less_le signed.not_less word_sle_rbl)
 
 text \<open>Lemmas for unpacking \<^term>\<open>rev (to_bl n)\<close> for numerals n and also
   for irreducible values and expressions.\<close>
@@ -447,6 +422,7 @@ fun nat_get_Suc_simproc_fn n_sucs ctxt ct =
 fun nat_get_Suc_simproc n_sucs ts =
   Simplifier.make_simproc \<^context>
    {name = "nat_get_Suc",
+    kind = Simproc,
     lhss = map (fn t => t $ \<^term>\<open>n :: nat\<close>) ts,
     proc = K (nat_get_Suc_simproc_fn n_sucs),
     identifier = []};
