lib/Word_Lib/Typedef_Morphisms.thy
@@ -2,6 +2,7 @@
  * Copyright Data61, CSIRO (ABN 41 687 119 230)
  *
  * SPDX-License-Identifier: BSD-2-Clause
+Proofs tidied by LCP, 2024-09
  *)
 
 (*
@@ -13,7 +14,7 @@
 section \<open>Type Definition Theorems\<close>
 
 theory Typedef_Morphisms
-  imports Main "HOL-Library.Word" Bit_Comprehension Bits_Int
+  imports Main "HOL-Library.Word" More_Int Bit_Comprehension
 begin
 
 subsection "More lemmas about normal type definitions"
@@ -96,16 +97,24 @@ subsection "Extended form of type definition predicate"
 lemma td_conds:
   "norm \<circ> norm = norm \<Longrightarrow>
     fr \<circ> norm = norm \<circ> fr \<longleftrightarrow> norm \<circ> fr \<circ> norm = fr \<circ> norm \<and> norm \<circ> fr \<circ> norm = norm \<circ> fr"
-  apply safe
-    apply (simp_all add: comp_assoc)
-   apply (simp_all add: o_assoc)
-  done
+  by (metis fun.map_comp)
 
-lemma fn_comm_power: "fa \<circ> tr = tr \<circ> fr \<Longrightarrow> fa ^^ n \<circ> tr = tr \<circ> fr ^^ n"
-  apply (rule ext)
-  apply (induct n)
-   apply (auto dest: fun_cong)
-  done
+lemma fn_comm_power: 
+  assumes "fa \<circ> tr = tr \<circ> fr"
+  shows "fa ^^ n \<circ> tr = tr \<circ> fr ^^ n"
+proof -
+  have "\<And>x. (fa ^^ n) (tr x) = tr ((fr ^^ n) x)"
+  proof (induction n)
+    case 0
+    then show ?case by auto
+  next
+    case (Suc n)
+    then show ?case
+      by (metis assms comp_def funpow.simps(2))
+  qed
+  then show ?thesis
+    by force
+qed
 
 lemmas fn_comm_power' =
   ext [THEN fn_comm_power, THEN fun_cong, unfolded o_def]
@@ -117,16 +126,16 @@ locale td_ext = type_definition +
 begin
 
 lemma Abs_norm [simp]: "Abs (norm x) = Abs x"
-  using eq_norm [of x] by (auto elim: Rep_inverse')
+  using Rep_inverse' eq_norm by blast
 
 lemma td_th: "g \<circ> Abs = f \<Longrightarrow> f (Rep x) = g x"
-  by (drule comp_Abs_inverse [symmetric]) simp
+  by auto
 
 lemma eq_norm': "Rep \<circ> Abs = norm"
   by (auto simp: eq_norm)
 
 lemma norm_Rep [simp]: "norm (Rep x) = Rep x"
-  by (auto simp: eq_norm' intro: td_th)
+  using eq_norm' td_th by force
 
 lemmas td = td_thm
 
@@ -134,10 +143,7 @@ lemma set_iff_norm: "w \<in> A \<longleftrightarrow> w = norm w"
   by (auto simp: set_Rep_Abs eq_norm' eq_norm [symmetric])
 
 lemma inverse_norm: "Abs n = w \<longleftrightarrow> Rep w = norm n"
-  apply (rule iffI)
-   apply (clarsimp simp add: eq_norm)
-  apply (simp add: eq_norm' [symmetric])
-  done
+  by (metis Rep_inverse eq_norm)
 
 lemma norm_eq_iff: "norm x = norm y \<longleftrightarrow> Abs x = Abs y"
   by (simp add: eq_norm' [symmetric])
@@ -164,36 +170,13 @@ text \<open>
   \<^item> \<open>norm \<circ> fr = fr\<close> says that \<open>fr\<close> takes any argument to a normalised result
 \<close>
 lemma fns2: "Abs \<circ> fr \<circ> Rep = fa \<Longrightarrow> norm \<circ> fr \<circ> norm = fr \<circ> norm \<longleftrightarrow> Rep \<circ> fa = fr \<circ> Rep"
-  apply (fold eq_norm')
-  apply safe
-   prefer 2
-   apply (simp add: o_assoc)
-  apply (rule ext)
-  apply (drule_tac x="Rep x" in fun_cong)
-  apply auto
-  done
+  by (metis (no_types, lifting) comp_Abs_inverse comp_assoc eq_norm')
 
 lemma fns3: "Abs \<circ> fr \<circ> Rep = fa \<Longrightarrow> norm \<circ> fr \<circ> norm = norm \<circ> fr \<longleftrightarrow> fa \<circ> Abs = Abs \<circ> fr"
-  apply (fold eq_norm')
-  apply safe
-   prefer 2
-   apply (simp add: comp_assoc)
-  apply (rule ext)
-  apply (drule_tac f="a \<circ> b" for a b in fun_cong)
-  apply simp
-  done
+  by (metis (no_types, lifting) eq_norm' fun.map_comp norm_norm(1))
 
 lemma fns: "fr \<circ> norm = norm \<circ> fr \<Longrightarrow> fa \<circ> Abs = Abs \<circ> fr \<longleftrightarrow> Rep \<circ> fa = fr \<circ> Rep"
-  apply safe
-   apply (frule fns1b)
-   prefer 2
-   apply (frule fns1a)
-   apply (rule fns3 [THEN iffD1])
-     prefer 3
-     apply (rule fns2 [THEN iffD1])
-       apply (simp_all add: comp_assoc)
-   apply (simp_all add: o_assoc)
-  done
+  by (metis (mono_tags, lifting) eq_norm' fns2 fns4 fun.map_comp norm_norm(1))
 
 lemma range_norm: "range (Rep \<circ> Abs) = A"
   by (simp add: set_Rep_Abs)
@@ -224,11 +207,8 @@ definition unats :: "nat \<Rightarrow> nat set"
 
 \<comment> \<open>naturals\<close>
 lemma uints_unats: "uints n = int ` unats n"
-  apply (unfold unats_def uints_num)
-  apply safe
-    apply (rule_tac image_eqI)
-     apply (erule_tac nat_0_le [symmetric])
-  by auto
+  unfolding unats_def uints_num
+  using nonneg_int_cases by fastforce
 
 lemma unats_uints: "unats n = nat ` uints n"
   by (auto simp: uints_unats image_iff)
@@ -236,10 +216,8 @@ lemma unats_uints: "unats n = nat ` uints n"
 lemma td_ext_uint:
   "td_ext (uint :: 'a word \<Rightarrow> int) word_of_int (uints (LENGTH('a::len)))
     (\<lambda>w::int. w mod 2 ^ LENGTH('a))"
-  apply (unfold td_ext_def')
-  apply transfer
-  apply (simp add: uints_num take_bit_eq_mod)
-  done
+  unfolding td_ext_def'
+  by transfer (simp add: uints_num take_bit_eq_mod)
 
 interpretation word_uint:
   td_ext
@@ -255,10 +233,7 @@ lemmas int_word_uint = word_uint.eq_norm
 lemma td_ext_ubin:
   "td_ext (uint :: 'a word \<Rightarrow> int) word_of_int (uints (LENGTH('a::len)))
     (take_bit (LENGTH('a)))"
-  apply standard
-  apply transfer
-  apply simp
-  done
+  by (simp add: td_ext_axioms.intro td_ext_def td_uint uint_word_of_int_eq)
 
 interpretation word_ubin:
   td_ext
@@ -271,10 +246,7 @@ interpretation word_ubin:
 lemma td_ext_unat [OF refl]:
   "n = LENGTH('a::len) \<Longrightarrow>
     td_ext (unat :: 'a word \<Rightarrow> nat) of_nat (unats n) (\<lambda>i. i mod 2 ^ n)"
-  apply (standard; transfer)
-     apply (simp_all add: unats_def take_bit_of_nat take_bit_nat_eq_self_iff
-      flip: take_bit_eq_mod)
-  done
+  by (simp add: td_ext_def' unat_of_nat unats_def)
 
 lemmas unat_of_nat = td_ext_unat [THEN td_ext.eq_norm]
 
@@ -290,10 +262,7 @@ lemmas td_unat = word_unat.td_thm
 
 lemma unat_le: "y \<le> unat z \<Longrightarrow> y \<in> unats (LENGTH('a))"
   for z :: "'a::len word"
-  apply (unfold unats_def)
-  apply clarsimp
-  apply (metis le_unat_uoi unsigned_less)
-  done
+  by (metis le_unat_uoi word_unat.Rep)
 
 lemma td_ext_sbin:
   "td_ext (sint :: 'a word \<Rightarrow> int) word_of_int (sints (LENGTH('a::len)))
@@ -355,21 +324,24 @@ interpretation test_bit:
 lemmas td_nth = test_bit.td_thm
 
 lemma sints_subset:
-  "m \<le> n \<Longrightarrow> sints m \<subseteq> sints n"
-  apply (simp add: sints_num)
-  apply clarsimp
-  apply (rule conjI)
-   apply (erule order_trans[rotated])
-   apply simp
-  apply (erule order_less_le_trans)
-  apply simp
-  done
+  assumes "m \<le> n"
+  shows "sints m \<subseteq> sints n"
+proof -
+  have "\<And>i::int. \<lbrakk>- (2 ^ (m - Suc 0)) \<le> i; i < 2 ^ (m - Suc 0)\<rbrakk>
+         \<Longrightarrow> - (2 ^ (n - Suc 0)) \<le> i"
+    by (smt (verit, ccfv_SIG) assms le_diff_conv power_increasing_iff)
+  moreover
+  have "\<And>i::int. \<lbrakk>- (2 ^ (m - Suc 0)) \<le> i; i < 2 ^ (m - Suc 0)\<rbrakk>
+         \<Longrightarrow> i < 2 ^ (n - Suc 0)"
+    using assms order_less_le_trans  by fastforce
+  ultimately show ?thesis
+    by (auto simp add: sints_num)
+qed
 
 lemma uints_mono_iff: "uints l \<subseteq> uints m \<longleftrightarrow> l \<le> m"
   using power_increasing_iff[of "2::int" l m]
-  apply (auto simp: uints_num subset_iff simp del: power_increasing_iff)
-  apply (meson less_irrefl not_le zero_le_numeral zero_le_power)
-  done
+  unfolding uints_num subset_iff mem_Collect_eq
+  by (smt (verit, best) not_exp_less_eq_0_int)
 
 lemmas uints_monoI = uints_mono_iff[THEN iffD2]
 
@@ -382,19 +354,30 @@ lemma Bit_in_uintsI: "of_bool c + 2 * w \<in> uints m" if "w \<in> uints (m - 1)
   by auto
 
 lemma bin_cat_in_uintsI:
-  \<open>concat_bit n b a \<in> uints m\<close> if \<open>a \<in> uints l\<close> \<open>m \<ge> l + n\<close>
+  \<open>concat_bit n b a \<in> uints m\<close> if \<open>a \<in> uints l\<close> \<open>l + n \<le> m\<close>
 proof -
-  from \<open>m \<ge> l + n\<close> obtain q where \<open>m = l + n + q\<close>
-    using le_Suc_ex by blast
-  then have \<open>(2::int) ^ m = 2 ^ n * 2 ^ (l + q)\<close>
-    by (simp add: ac_simps power_add)
-  moreover have \<open>a mod 2 ^ (l + q) = a\<close>
-    using \<open>a \<in> uints l\<close>
-    by (auto simp add: uints_def take_bit_eq_mod power_add Divides.mod_mult2_eq)
-  ultimately have \<open>concat_bit n b a = take_bit m (concat_bit n b a)\<close>
-    by (simp add: concat_bit_eq take_bit_eq_mod push_bit_eq_mult Divides.mod_mult2_eq)
-  then show ?thesis
-    by (simp add: uints_def)
+  from \<open>a \<in> uints l\<close> have \<open>0 \<le> a\<close> \<open>a < 2 ^ l\<close>
+    by (auto simp add: uints_def range_bintrunc)
+  define q where \<open>q = m - n\<close>
+  with \<open>l + n \<le> m\<close> have \<open>m = n + q\<close>
+    by simp
+  from \<open>q = m - n\<close> \<open>l + n \<le> m\<close> have \<open>l \<le> q\<close>
+    by simp
+  then have \<open>(2::int) ^ l \<le> 2 ^ q\<close>
+    by simp
+  with \<open>a < 2 ^ l\<close> have \<open>a < 2 ^ q\<close>
+    by linarith
+  have \<open>take_bit n b < 2 ^ n * 2 ^ q\<close>
+    using take_bit_int_less_exp [of n b]
+    by (rule order.strict_trans2) simp
+  then have \<open>take_bit n b < 2 ^ (n + q)\<close>
+    by (simp add: power_add)
+  moreover have \<open>push_bit n a < 2 ^ (n + q)\<close>
+    using \<open>a < 2 ^ q\<close> by (simp add: power_add push_bit_eq_mult)
+  ultimately have \<open>concat_bit n b a < 2 ^ (n + q)\<close>
+    by (simp add: concat_bit_def OR_upper)
+  with \<open>0 \<le> a\<close> show ?thesis
+    by (simp add: uints_def range_bintrunc \<open>m = n + q\<close>)
 qed
 
 end
